initial exceptions proof

Final/Basic.lean
@@ -1,1 +1,413 @@
-def hello := "world"
+-- syntax and semantics: top-level functions + tuples + exceptions
+
+abbrev Var := String
+
+inductive Expr where
+  | int (i : Int) : Expr
+  | succ (e : Expr) : Expr
+  | pred (e : Expr) : Expr
+  | plus (e1 : Expr) (e2 : Expr) : Expr
+  | times (e1 : Expr) (e3 : Expr) : Expr
+  | ifte (e1 e2 e3 : Expr) : Expr
+  | bool (b : Bool) : Expr
+  | neg (e : Expr) : Expr
+  | bind (x : Var) (e1 e2 : Expr) : Expr
+  | var (x : Var) : Expr
+  | call (f : Var) (e : Expr) : Expr
+  | pair (e1 e2 : Expr) : Expr
+  | fst (e : Expr) : Expr
+  | snd (e : Expr) : Expr
+  | throw (e : Expr) : Expr
+  | handle (e : Expr) (f : Var) : Expr
+
+inductive Defn where
+  | defn (f x : Var) (e : Expr)
+
+inductive Val where
+  | int (i : Int) : Val
+  | bool (b : Bool) : Val
+  | pair (v1 v2 : Val)
+
+inductive Ans where
+  | val (v : Val) : Ans
+  | exn (v : Val) : Ans
+
+abbrev Env := List (Var × Val)
+
+abbrev Defns := List Defn
+
+abbrev Prog := Defns × Expr
+
+def Env.lookup (r : Env) (x : Var) : Option Val :=
+  match r with
+  | [] => none
+  | (y,v) :: r =>
+    if x = y then some v else Env.lookup r x
+
+def Defns.lookup (ds : Defns) (f : Var) : Option Defn :=
+  match ds with
+  | [] => none
+  | ((.defn g y e) :: ds) =>
+    if f = g then some (.defn g y e) else Defns.lookup ds f
+
+inductive Eval : Defns → Env → Expr → Ans → Prop where
+  | intr {ds r} (i : Int) :
+    Eval ds r (.int i) (.val (.int i))
+  | boolr {ds r} (b : Bool) :
+    Eval ds r (.bool b) (.val (.bool b))
+  | succr {ds r e i} :
+    Eval ds r e (.val (.int i)) →
+    Eval ds r (.succ e) (.val (.int (i + 1)))
+  | succ_propr {ds r e v} :
+    Eval ds r e (.exn v) →
+    Eval ds r (.succ e) (.exn v)
+  | predr {ds r e i} :
+    Eval ds r e (.val (.int i)) →
+    Eval ds r (.pred e) (.val (.int (i - 1)))
+  | pred_propr {ds r e v} :
+    Eval ds r e (.exn v) →
+    Eval ds r (.pred e) (.exn v)
+  | plusr {ds r e1 i1 e2 i2} :
+    Eval ds r e1 (.val (.int i1)) →
+    Eval ds r e2 (.val (.int i2)) →
+    Eval ds r (.plus e1 e2) (.val (.int (i1 + i2)))
+  | plus_proplr {ds r e1 v e2} :
+    Eval ds r e1 (.exn v) →
+    Eval ds r (.plus e1 e2) (.exn v)
+  | plus_proprr {ds r e1 e2 v1 v2} :
+    Eval ds r e1 (.val v1) →
+    Eval ds r e2 (.exn v2) →
+    Eval ds r (.plus e1 e2) (.exn v2)
+  | timesr {ds r e1 i1 e2 i2} :
+    Eval ds r e1 (.val (.int i1)) →
+    Eval ds r e2 (.val (.int i2)) →
+    Eval ds r (.times e1 e2) (.val (.int (i1 * i2)))
+  | times_proplr {ds r e1 v e2} :
+    Eval ds r e1 (.exn v) →
+    Eval ds r (.times e1 e2) (.exn v)
+  | times_proprr {ds r e1 e2 v1 v2} :
+    Eval ds r e1 (.val v1) →
+    Eval ds r e2 (.exn v2) →
+    Eval ds r (.times e1 e2) (.exn v2)
+  | iftr {ds r e1 e2 a e3} :
+    Eval ds r e1 (.val (.bool true)) →
+    Eval ds r e2 a →
+    Eval ds r (.ifte e1 e2 e3) a
+  | iffr {ds r e1 e3 a e2} :
+    Eval ds r e1 (.val (.bool false)) →
+    Eval ds r e3 a →
+    Eval ds r (.ifte e1 e2 e3) a
+  | if_propr {ds r e1 v e2 e3} :
+    Eval ds r e1 (.exn v) →
+    Eval ds r (.ifte e1 e2 e3) (.exn v)
+  | negtr {ds r e} :
+    Eval ds r e (.val (.bool true)) →
+    Eval ds r (.neg e) (.val (.bool false))
+  | negfr {ds r e} :
+    Eval ds r e (.val (.bool false)) →
+    Eval ds r (.neg e) (.val (.bool true))
+  | neg_propr {ds r e v} :
+    Eval ds r e (.exn v) →
+    Eval ds r (.neg e) (.exn v)
+  | varr {ds r v x} :
+    Env.lookup r x = some v →
+    Eval ds r (.var x) (.val v)
+  | bindr {ds r e1 v1 x a e2} :
+    Eval ds r e1 (.val v1) →
+    Eval ds ((x, v1) :: r) e2 a →
+    Eval ds r (.bind x e1 e2) a
+  | bind_propr {ds r e1 v x e2} :
+    Eval ds r e1 (.exn v) →
+    Eval ds r (.bind x e1 e2) (.exn v)
+  | callr {ds r e v1 f x e' a} :
+    Eval ds r e (.val v1) →
+    Defns.lookup ds f = some (.defn f x e') →
+    Eval ds [(x,v1)] e' a →
+    Eval ds r (.call f e) a
+  | call_propr {ds r e f v} :
+    Eval ds r e (.exn v) →
+    Eval ds r (.call f e) (.exn v)
+  | pairr {ds r e1 v1 e2 v2} :
+    Eval ds r e1 (.val v1) →
+    Eval ds r e2 (.val v2) →
+    Eval ds r (.pair e1 e2) (.val (.pair v1 v2))
+  | pair_proplr {ds r e1 v e2} :
+    Eval ds r e1 (.exn v) →
+    Eval ds r (.pair e1 e2) (.exn v)
+  | pair_proprr {ds r e1 e2 v1 v2} :
+    Eval ds r e1 (.val v1) →
+    Eval ds r e2 (.exn v2) →
+    Eval ds r (.pair e1 e2) (.exn v2)
+  | fstr {ds r e v1 v2} :
+    Eval ds r e (.val (.pair v1 v2)) →
+    Eval ds r (.fst e) (.val v1)
+  | fst_propr {ds r e v} :
+    Eval ds r e (.exn v) →
+    Eval ds r (.fst e) (.exn v)
+  | sndr {ds r e v1 v2} :
+    Eval ds r e (.val (.pair v1 v2)) →
+    Eval ds r (.snd e) (.val v2)
+  | snd_propr {ds r e v} :
+    Eval ds r e (.exn v) →
+    Eval ds r (.snd e) (.exn v)
+  | throwr {ds r e v} :
+    Eval ds r e (.val v) →
+    Eval ds r (.throw e) (.exn v)
+  | throw_propr {ds r e v} :
+    Eval ds r e (.exn v) →
+    Eval ds r (.throw e) (.exn v)
+  | handle_valr {ds r e v f} :
+    Eval ds r e (.val v) →
+    Eval ds r (.handle e f) (.val v)
+  | handle_exnr {ds r e v f x e' a} :
+    Eval ds r e (.exn v) →
+    Defns.lookup ds f = some (.defn f x e') →
+    Eval ds [(x,v)] e' a →
+    Eval ds r (.handle e f) a
+
+
+-- A little stack machine semantics
+
+inductive Op where
+| plus | times | flip
+
+inductive Instr where
+| push (i : Int) : Instr
+| op (o : Op) : Instr
+| branch (is1 is2 : List Instr)
+| get (n : Nat) : Instr
+| pop : Instr
+| exch : Instr
+| call : Instr
+| dup : Instr
+| alloc (n : Nat) : Instr
+| read (o : Int) : Instr
+| write (o : Int) : Instr
+| trycatch (is1 is2 : List Instr) : Instr
+| abort : Instr
+
+abbrev Instrs := List Instr
+
+abbrev Stack := List Int
+
+abbrev IDefns := List Instrs
+
+inductive OpEval : Op → List Int → Int → Prop where
+| flip0 : OpEval .flip [0] 1
+| flip1 : OpEval .flip [1] 0
+| plus {i j} : OpEval .plus [j, i] (i+j)
+| mult {i j} : OpEval .times [j, i] (i*j)
+
+abbrev Heap := List (Int × Int)
+
+def Heap.lookup (h : Heap) (i : Int) : Option Int :=
+  match h with
+  | [] => none
+  | (j,k) :: h =>
+    if i = j then some k else Heap.lookup h i
+
+def Heap.ext (h : Heap) (i j : Int) : Heap :=
+  (i, j) :: h
+
+def FreshBlock (h : Heap) (base : Int) (n : Nat) : Prop :=
+  ∀ k : Nat, k < n → Heap.lookup h (base + Int.ofNat k) = none
+
+inductive Frame where
+  | ret (is : Instrs)
+  | handler (handler : Instrs) (k : Instrs)
+
+inductive Step : IDefns →
+                 Instrs → List Frame → Stack → Heap →
+                 Instrs → List Frame → Stack → Heap → Prop where
+| pushr {ds v is cs s h} :
+  Step ds (.push v :: is) cs s h is cs (v :: s) h
+| opr {ds o vs v is cs s h} : OpEval o vs v →
+  Step ds (.op o :: is) cs (vs ++ s) h is cs (v :: s) h
+| branchtr {ds is1 is2 is cs s h} :
+  Step ds (.branch is1 is2 :: is) cs (1 :: s) h (is1 ++ is) cs s h
+| branchfr {ds is1 is2 is cs s h} :
+  Step ds (.branch is1 is2 :: is) cs (0 :: s) h (is2 ++ is) cs s h
+| popr {ds is cs i s h} :
+  Step ds (.pop :: is) cs (i :: s) h is cs s h
+| getr {ds n is cs s h i} :
+  s[n]? = some i →
+  Step ds (.get n :: is) cs s h is cs (i :: s) h
+| exchr {ds is cs v1 v2 s h} :
+  Step ds (.exch :: is) cs (v1 :: v2 :: s) h is cs (v2 :: v1 :: s) h
+| callr {ds i is' is cs s h} :
+  ds[i.toNat]? = some is' →
+  Step ds (.call :: is) cs (i :: s) h (is' ++ is) cs s h
+| dupr {ds is cs i s h} :
+  Step ds (.dup :: is) cs (i :: s) h is cs (i :: i :: s) h
+| allocr {ds is cs s h n i} :
+  FreshBlock h i n →
+  Step ds (.alloc n :: is) cs s h is cs (i :: s) h
+| readr {ds h i j o is cs s} :
+  Heap.lookup h (i + o) = some j →
+  Step ds (.read o :: is) cs (i :: s) h is cs (j :: s) h
+| writer {ds is cs i j o s h} :
+  Step ds (.write o :: is) cs (i :: j :: s) h is cs (i :: s) (Heap.ext h (i + o) j)
+| trycatchr {ds is body handle cs s h} :
+  Step ds (.trycatch body handle :: is) cs s h
+    body (.handler handle is :: cs) s h
+| ret_handler {ds handle k cs s h} :
+  Step ds [] (.handler handle k :: cs) s h k cs s h
+| abort_handler {ds is' handle k cs s h} :
+  Step ds (.abort :: is') (.handler handle k :: cs) s h handle (.ret k :: cs) s h
+| abort_retr {ds is' k cs s h} :
+  Step ds (.abort :: is') (.ret k :: cs) s h (.abort :: is') cs s h
+| retr {ds is cs s h} :
+  Step ds [] (.ret is :: cs) s h is cs s h
+
+inductive Steps : IDefns →
+  Instrs → List Frame → Stack → Heap →
+  Instrs → List Frame → Stack → Heap → Prop where
+| refl {ds s is cs h} : Steps ds is cs s h is cs s h
+| trans {ds is cs s h is1 cs1 s1 h1 is' cs' s' h'} :
+  Steps ds is cs s h is1 cs1 s1 h1 ->
+  Step ds is1 cs1 s1 h1 is' cs' s' h' ->
+  Steps ds is cs s h is' cs' s' h'
+
+-- compiler
+
+abbrev CEnv := List (Option Var)
+
+def CEnv.lookup (c : CEnv) (x : Var) : Option Nat :=
+  match c with
+  | [] => none
+  | some y :: c =>
+    if x = y then some 0 else
+      (CEnv.lookup c x).map .succ
+  | none :: c =>
+      (CEnv.lookup c x).map .succ
+
+def Defns.indexOf (ds : Defns) (f : Var) : Option Nat :=
+  match ds with
+  | [] => none
+  | (.defn g _ _) :: ds =>
+    if f = g then some 0 else (indexOf ds f).map .succ
+
+def compile (ds : Defns) (c : CEnv) (e : Expr) : List Instr :=
+  match e with
+  | .int i => [.push i]
+  | .bool b => [.push (if b then 1 else 0)]
+  | .succ e =>
+    compile ds c e ++
+    [.push 1, .op .plus]
+  | .pred e =>
+    compile ds c e ++
+    [.push (-1), .op .plus]
+  | .neg e =>
+    compile ds c e ++
+    [.op .flip]
+  | .plus e1 e2 =>
+    compile ds c e1 ++
+    compile ds (none :: c) e2 ++
+    [.op .plus]
+  | .times e1 e2 =>
+    compile ds c e1 ++
+    compile ds (none :: c) e2 ++
+    [.op .times]
+  | .ifte e1 e2 e3 =>
+    compile ds c e1 ++
+    [.branch (compile ds c e2) (compile ds c e3)]
+  | .var x =>
+    match CEnv.lookup c x with
+    | some n =>
+      [.get n]
+    | none => [] -- whatever
+  | .bind x e1 e2 =>
+    compile ds c e1 ++
+    compile ds (some x :: c) e2 ++
+    [.exch, .pop]
+  | .call f e =>
+    compile ds c e ++
+    match Defns.indexOf ds f with
+    | some n => [.push (Int.ofNat n), .call, .exch, .pop]
+    | none => [] -- whatever
+  | .pair e1 e2 =>
+    compile ds c e1 ++
+    compile ds (none :: c) e2 ++
+    [.alloc 2, .write 1, .write 0]
+  | .fst e =>
+    compile ds c e ++
+    [.read 0]
+  | .snd e =>
+    compile ds c e ++
+    [.read 1]
+  | .throw e =>
+    compile ds c e ++
+    [.abort]
+  | .handle e f =>
+    [.trycatch (compile ds c e)
+      (match Defns.indexOf ds f with
+       | some n => [.push (Int.ofNat n), .call, .exch, .pop]
+       | none   => [])]
+
+def compile_defn (ds : Defns) (d : Defn) :=
+  match d with
+  | .defn _ x e => compile ds [some x] e
+
+def compile_defns (ds : Defns) :=
+  ds.map (compile_defn ds)
+
+-- proof
+
+inductive Represents : Val -> Int -> Heap -> Prop where
+  | int {i h} : Represents (.int i) i h
+  | bool {b h} : Represents (.bool b) (if b then 1 else 0) h
+  | pair {v1 i1 h v2 i2 i} :
+    Represents v1 i1 h ->
+    Represents v2 i2 h ->
+    Heap.lookup h (i+0) = i1 ->
+    Heap.lookup h (i+1) = i2 ->
+    Represents (.pair v1 v2) i h
+
+inductive Related : Stack -> CEnv -> Env -> Heap -> Prop where
+  | mt {s h} : Related s [] [] h
+  | push {s c r i h} :
+    Related s c r h ->
+    Related (i :: s) (none :: c) r h
+  | bind {s c r x v h i} :
+    Related s c r h ->
+    Represents v i h ->
+    Related (i :: s) ((some x) :: c) ((x,v) :: r) h
+
+def AnsRep : Ans → Int → Heap → Prop
+  | .val v, i, h => Represents v i h
+  | .exn v, i, h => Represents v i h
+
+-- * values return normally;
+-- * exceptions skip .ret frames;
+-- * exceptions jump to the nearest .handler;
+-- * if there is no handler, they leave the machine at (.abort :: is).
+inductive ContinuesWith :
+  Ans → Instrs → List Frame → Stack →
+  Int → Instrs → List Frame → Stack → Prop where
+| val {v is cs s i} :
+  ContinuesWith (.val v) is cs s i
+    is cs (i :: s)
+| exn_nil {v is s i} :
+  ContinuesWith (.exn v) is [] s i
+    (.abort :: is) [] (i :: s)
+| exn_ret {v is k cs s i is' cs' s'} :
+  ContinuesWith (.exn v) is cs s i is' cs' s' →
+  ContinuesWith (.exn v) is (.ret k :: cs) s i is' cs' s'
+| exn_handler {v is handle k cs s i} :
+  ContinuesWith (.exn v) is (.handler handle k :: cs) s i
+    handle (.ret k :: cs) (i :: s)
+
+def HeapExtends (h h' : Heap) : Prop :=
+  ∀ a v,
+  Heap.lookup h a = some v ->
+  Heap.lookup h' a = some v
+
+theorem compiler_correct_general
+  {ds c r e a is cs s h} :
+  Related s c r h →
+  Eval ds r e a →
+  ∃ i h' is' cs' s',
+    Steps (compile_defns ds) (compile ds c e ++ is) cs s h is' cs' s' h' ∧
+    ContinuesWith a is cs s i is' cs' s' ∧
+    AnsRep a i h' ∧
+    HeapExtends h h' := by sorry
